src/Comparse.Tests.TacticFeatures.fst
@@ -192,6 +192,24 @@ let test_match_parser bytes #bl n =
 %splice [ps_test_match_parser] (gen_parser (`test_match_parser))
 #pop-options
 
+[@@ can_be_unit]
+val test_unit_match_parser: bytes:Type0 -> {|bytes_like bytes|} -> n:nat -> Type0
+let test_unit_match_parser bytes #bl n =
+  let n2 = nat_func_1 n in
+  match nat_func_2 (nat_func_3 n) with
+  | 0 -> unit
+  | 1 -> test_ne
+  | 2 -> test_ii #bytes
+  | 3 -> test_ie #bytes
+  | 4 -> test_ei bytes
+  | 5 -> test_ee bytes
+  | 6 -> if nat_pred_1 n2 then test_dep_nat_n n2 else test_dep_nat_e bytes (n2+42)
+  | _ -> test_dep_nat_i #bytes (nat_func_4 n2)
+
+#push-options "--fuel 0 --ifuel 0"
+%splice [ps_test_unit_match_parser] (gen_parser (`test_unit_match_parser))
+#pop-options
+
 type test_tag_unit =
   | TagUnit1: unit -> test_tag_unit
   | TagUnit2: unit -> test_tag_unit
@@ -478,7 +496,6 @@ noeq type test_dependent_sum (bytes:Type0) {|bytes_like bytes|} =
 #push-options "--fuel 0 --ifuel 1 --z3cliopt 'smt.qi.eager_threshold=0' --z3rlimit 50"
 %splice [ps_test_dependent_sum_serialize] (gen_serialize_lemma (`test_dependent_sum))
 #pop-options
-
 
 (*** Stress test ***)
 
